add bottom and lower bounds, requires trans pushback

stable/FsubL.v
@@ -1,12 +1,27 @@
 (***************************************************************************
-* Preservation and Progress for System-F with Subtyping - Definitions      *
-* Brian Aydemir & Arthur Charguéraud, March 2007                           *
+  Preservation and Progress for System-F
+  with Subtyping, Bottom and Lower Bounds
+
+- based on the POPLMark solution of
+  Brian Aydemir & Arthur Charguéraud, March 2007
+  cf. https://github.com/samuelgruetter/dot-calculus/blob/master/ln/Fsub_Definitions.v
+  cf. https://github.com/samuelgruetter/dot-calculus/blob/master/ln/Fsub_Infrastructure.v
+  cf. https://github.com/samuelgruetter/dot-calculus/blob/master/ln/Fsub_Part1A.v
+
+- transitivity pushback based on ideas by Tiark Rompf
+  and implementation by Samuel Gruetter,
+  cf. https://github.com/samuelgruetter/dot-calculus/blob/master/stable/DotTransitivity-SingleDecBind.v
+
 ***************************************************************************)
 
 Set Implicit Arguments.
 Require Import LibLN.
 Implicit Types x : var.
 Implicit Types X : var.
+
+(***************************************************************************
+* Definitions                                                              *
+***************************************************************************)
 
 (* ********************************************************************** *)
 (** * Description of the Language *)
@@ -15,10 +30,11 @@ Implicit Types X : var.
 
 Inductive typ : Set :=
   | typ_top   : typ
+  | typ_bot   : typ
   | typ_bvar  : nat -> typ
   | typ_fvar  : var -> typ
   | typ_arrow : typ -> typ -> typ
-  | typ_all   : typ -> typ -> typ.
+  | typ_all   : typ -> typ -> typ -> typ.
 
 (** Representation of pre-terms *)
 
@@ -27,7 +43,7 @@ Inductive trm : Set :=
   | trm_fvar : var -> trm
   | trm_abs  : typ -> trm -> trm
   | trm_app  : trm -> trm -> trm
-  | trm_tabs : typ -> trm -> trm
+  | trm_tabs : typ -> typ -> trm -> trm
   | trm_tapp : trm -> typ -> trm.
 
 (** Opening up a type binder occuring in a type *)
@@ -35,10 +51,11 @@ Inductive trm : Set :=
 Fixpoint open_tt_rec (K : nat) (U : typ) (T : typ) {struct T} : typ :=
   match T with
   | typ_top         => typ_top
+  | typ_bot         => typ_bot
   | typ_bvar J      => If K = J then U else (typ_bvar J)
   | typ_fvar X      => typ_fvar X
   | typ_arrow T1 T2 => typ_arrow (open_tt_rec K U T1) (open_tt_rec K U T2)
-  | typ_all T1 T2   => typ_all (open_tt_rec K U T1) (open_tt_rec (S K) U T2)
+  | typ_all T0 T1 T2   => typ_all (open_tt_rec K U T0) (open_tt_rec K U T1) (open_tt_rec (S K) U T2)
   end.
 
 Definition open_tt T U := open_tt_rec 0 U T.
@@ -51,7 +68,7 @@ Fixpoint open_te_rec (K : nat) (U : typ) (e : trm) {struct e} : trm :=
   | trm_fvar x    => trm_fvar x
   | trm_abs V e1  => trm_abs  (open_tt_rec K U V)  (open_te_rec K U e1)
   | trm_app e1 e2 => trm_app  (open_te_rec K U e1) (open_te_rec K U e2)
-  | trm_tabs V e1 => trm_tabs (open_tt_rec K U V)  (open_te_rec (S K) U e1)
+  | trm_tabs VS VU e1 => trm_tabs (open_tt_rec K U VS) (open_tt_rec K U VU)  (open_te_rec (S K) U e1)
   | trm_tapp e1 V => trm_tapp (open_te_rec K U e1) (open_tt_rec K U V)
   end.
 
@@ -65,7 +82,7 @@ Fixpoint open_ee_rec (k : nat) (f : trm) (e : trm) {struct e} : trm :=
   | trm_fvar x    => trm_fvar x
   | trm_abs V e1  => trm_abs V (open_ee_rec (S k) f e1)
   | trm_app e1 e2 => trm_app (open_ee_rec k f e1) (open_ee_rec k f e2)
-  | trm_tabs V e1 => trm_tabs V (open_ee_rec k f e1)
+  | trm_tabs VS VU e1 => trm_tabs VS VU (open_ee_rec k f e1)
   | trm_tapp e1 V => trm_tapp (open_ee_rec k f e1) V
   end.
 
@@ -82,16 +99,19 @@ Notation "t 'open_ee_var' x" := (open_ee t (trm_fvar x)) (at level 67).
 Inductive type : typ -> Prop :=
   | type_top :
       type typ_top
+  | type_bot :
+      type typ_bot
   | type_var : forall X,
       type (typ_fvar X)
   | type_arrow : forall T1 T2,
       type T1 ->
       type T2 ->
       type (typ_arrow T1 T2)
-  | type_all : forall L T1 T2,
+  | type_all : forall L T0 T1 T2,
+      type T0 ->
       type T1 ->
       (forall X, X \notin L -> type (T2 open_tt_var X)) ->
-      type (typ_all T1 T2).
+      type (typ_all T0 T1 T2).
 
 (** Terms as locally closed pre-terms *)
 
@@ -106,27 +126,21 @@ Inductive term : trm -> Prop :=
       term e1 ->
       term e2 ->
       term (trm_app e1 e2)
-  | term_tabs : forall L V e1,
-      type V ->
+  | term_tabs : forall L VS VU e1,
+      type VS ->
+      type VU ->
       (forall X, X \notin L -> term (e1 open_te_var X)) ->
-      term (trm_tabs V e1)
+      term (trm_tabs VS VU e1)
   | term_tapp : forall e1 V,
       term e1 ->
       type V ->
       term (trm_tapp e1 V).
 
-(** Binding are either mapping type or term variables.
- [X ~<: T] is a subtyping asumption and [x ~: T] is
- a typing assumption *)
+(** Binding are either mapping type or term variables. *)
 
 Inductive bind : Set :=
-  | bind_sub : typ -> bind
+  | bind_sub : typ -> typ -> bind
   | bind_typ : typ -> bind.
-
-Notation "X ~<: T" := (X ~ bind_sub T)
-  (at level 23, left associativity) : env_scope.
-Notation "x ~: T" := (x ~ bind_typ T)
-  (at level 23, left associativity) : env_scope.
 
 (** Environment is an associative list of bindings. *)
 
@@ -140,18 +154,21 @@ Definition env := LibEnv.env bind.
 Inductive wft : env -> typ -> Prop :=
   | wft_top : forall E,
       wft E typ_top
-  | wft_var : forall U E X,
-      binds X (bind_sub U) E ->
+  | wft_bot : forall E,
+      wft E typ_bot
+  | wft_var : forall T0 T1 E X,
+      binds X (bind_sub T0 T1) E ->
       wft E (typ_fvar X)
   | wft_arrow : forall E T1 T2,
       wft E T1 ->
       wft E T2 ->
       wft E (typ_arrow T1 T2)
-  | wft_all : forall L E T1 T2,
+  | wft_all : forall L E T0 T1 T2,
+      wft E T0 ->
       wft E T1 ->
       (forall X, X \notin L ->
-        wft (E & X ~<: T1) (T2 open_tt_var X)) ->
-      wft E (typ_all T1 T2).
+        wft (E & X ~ bind_sub T0 T1) (T2 open_tt_var X)) ->
+      wft E (typ_all T0 T1 T2).
 
 (** A environment E is well-formed if it contains no duplicate bindings
   and if each type in it is well-formed with respect to the environment
@@ -160,35 +177,62 @@ Inductive wft : env -> typ -> Prop :=
 Inductive okt : env -> Prop :=
   | okt_empty :
       okt empty
-  | okt_sub : forall E X T,
-      okt E -> wft E T -> X # E -> okt (E & X ~<: T)
+  | okt_sub : forall E X T0 T1,
+      okt E -> wft E T0 -> wft E T1 -> X # E -> okt (E & X ~ bind_sub T0 T1)
   | okt_typ : forall E x T,
-      okt E -> wft E T -> x # E -> okt (E & x ~: T).
+      okt E -> wft E T -> x # E -> okt (E & x ~ bind_typ T).
 
 (** Subtyping relation *)
 
-Inductive sub : env -> typ -> typ -> Prop :=
+Inductive sub_mode : Set :=
+  | notrans : sub_mode
+  | oktrans : sub_mode.
+
+Inductive sub : sub_mode -> env -> typ -> typ -> Prop :=
   | sub_top : forall E S,
       okt E ->
       wft E S ->
-      sub E S typ_top
+      sub notrans E S typ_top
+  | sub_bot : forall E T,
+      okt E ->
+      wft E T ->
+      sub notrans E typ_bot T
   | sub_refl_tvar : forall E X,
       okt E ->
       wft E (typ_fvar X) ->
-      sub E (typ_fvar X) (typ_fvar X)
-  | sub_trans_tvar : forall U E T X,
-      binds X (bind_sub U) E ->
-      sub E U T ->
-      sub E (typ_fvar X) T
+      sub notrans E (typ_fvar X) (typ_fvar X)
+  | sub_trans_tvar : forall T0 T1 E T X,
+      binds X (bind_sub T0 T1) E ->
+      sub oktrans E T0 T1 ->
+      sub oktrans E T1 T ->
+      sub notrans E (typ_fvar X) T
+  | sub_trans_tvar_lower : forall T0 T1 E T X,
+      binds X (bind_sub T0 T1) E ->
+      sub oktrans E T0 T1 ->
+      sub oktrans E T T0 ->
+      sub notrans E T (typ_fvar X)
   | sub_arrow : forall E S1 S2 T1 T2,
-      sub E T1 S1 ->
-      sub E S2 T2 ->
-      sub E (typ_arrow S1 S2) (typ_arrow T1 T2)
-  | sub_all : forall L E S1 S2 T1 T2,
-      sub E T1 S1 ->
+      sub oktrans E T1 S1 ->
+      sub oktrans E S2 T2 ->
+      sub notrans E (typ_arrow S1 S2) (typ_arrow T1 T2)
+  | sub_refl_all : forall E T0 T1 T2,
+      okt E ->
+      wft E (typ_all T0 T1 T2) ->
+      sub notrans E (typ_all T0 T1 T2) (typ_all T0 T1 T2)
+  | sub_all : forall L E S0 S1 S2 T0 T1 T2,
+      sub oktrans E S0 T0 ->
+      sub oktrans E T1 S1 ->
+      sub oktrans E T0 T1 ->
       (forall X, X \notin L ->
-          sub (E & X ~<: T1) (S2 open_tt_var X) (T2 open_tt_var X)) ->
-      sub E (typ_all S1 S2) (typ_all T1 T2).
+          sub oktrans (E & X ~ bind_sub T0 T1) (S2 open_tt_var X) (T2 open_tt_var X)) ->
+      sub notrans E (typ_all S0 S1 S2) (typ_all T0 T1 T2)
+  | sub_trans_ok : forall E T1 T2,
+      sub notrans E T1 T2 ->
+      sub oktrans E T1 T2
+  | sub_trans : forall E T1 T2 T3,
+      sub oktrans E T1 T2 ->
+      sub oktrans E T2 T3 ->
+      sub oktrans E T1 T3.
 
 (** Typing relation *)
 
@@ -199,23 +243,25 @@ Inductive typing : env -> trm -> typ -> Prop :=
       typing E (trm_fvar x) T
   | typing_abs : forall L E V e1 T1,
       (forall x, x \notin L ->
-        typing (E & x ~: V) (e1 open_ee_var x) T1) ->
+        typing (E & x ~ bind_typ V) (e1 open_ee_var x) T1) ->
       typing E (trm_abs V e1) (typ_arrow V T1)
   | typing_app : forall T1 E e1 e2 T2,
       typing E e1 (typ_arrow T1 T2) ->
       typing E e2 T1 ->
       typing E (trm_app e1 e2) T2
-  | typing_tabs : forall L E V e1 T1,
+  | typing_tabs : forall L E VS VU e1 T1,
       (forall X, X \notin L ->
-        typing (E & X ~<: V) (e1 open_te_var X) (T1 open_tt_var X)) ->
-      typing E (trm_tabs V e1) (typ_all V T1)
-  | typing_tapp : forall T1 E e1 T T2,
-      typing E e1 (typ_all T1 T2) ->
-      sub E T T1 ->
+        typing (E & X ~ bind_sub VS VU) (e1 open_te_var X) (T1 open_tt_var X)) ->
+      sub oktrans E VS VU ->
+      typing E (trm_tabs VS VU e1) (typ_all VS VU T1)
+  | typing_tapp : forall T0 T1 E e1 T T2,
+      typing E e1 (typ_all T0 T1 T2) ->
+      sub oktrans E T0 T ->
+      sub oktrans E T T1 ->
       typing E (trm_tapp e1 T) (open_tt T2 T)
   | typing_sub : forall S E e T,
       typing E e S ->
-      sub E S T ->
+      sub oktrans E S T ->
       typing E e T.
 
 (** Values *)
@@ -223,8 +269,8 @@ Inductive typing : env -> trm -> typ -> Prop :=
 Inductive value : trm -> Prop :=
   | value_abs  : forall V e1, term (trm_abs V e1) ->
                  value (trm_abs V e1)
-  | value_tabs : forall V e1, term (trm_tabs V e1) ->
-                 value (trm_tabs V e1).
+  | value_tabs : forall VS VU e1, term (trm_tabs VS VU e1) ->
+                 value (trm_tabs VS VU e1).
 
 (** One-step reduction *)
 
@@ -245,10 +291,10 @@ Inductive red : trm -> trm -> Prop :=
       term (trm_abs V e1) ->
       value v2 ->
       red (trm_app (trm_abs V e1) v2) (open_ee e1 v2)
-  | red_tabs : forall V1 e1 V2,
-      term (trm_tabs V1 e1) ->
+  | red_tabs : forall V0 V1 e1 V2,
+      term (trm_tabs V0 V1 e1) ->
       type V2 ->
-      red (trm_tapp (trm_tabs V1 e1) V2) (open_te e1 V2).
+      red (trm_tapp (trm_tabs V0 V1 e1) V2) (open_te e1 V2).
 
 (** Our goal is to prove preservation and progress *)
 
@@ -263,7 +309,7 @@ Definition progress := forall e T,
   \/ exists e', red e e'.
 
 (***************************************************************************
-* Preservation and Progress for System-F with Subtyping - Infrastructure   *
+* Infrastructure                                                           *
 ***************************************************************************)
 
 (* ********************************************************************** *)
@@ -274,10 +320,11 @@ Definition progress := forall e T,
 Fixpoint fv_tt (T : typ) {struct T} : vars :=
   match T with
   | typ_top         => \{}
+  | typ_bot         => \{}
   | typ_bvar J      => \{}
   | typ_fvar X      => \{X}
   | typ_arrow T1 T2 => (fv_tt T1) \u (fv_tt T2)
-  | typ_all T1 T2   => (fv_tt T1) \u (fv_tt T2)
+  | typ_all T0 T1 T2   => (fv_tt T0) \u (fv_tt T1) \u (fv_tt T2)
   end.
 
 (** Computing free type variables in a term *)
@@ -288,7 +335,7 @@ Fixpoint fv_te (e : trm) {struct e} : vars :=
   | trm_fvar x    => \{}
   | trm_abs V e1  => (fv_tt V) \u (fv_te e1)
   | trm_app e1 e2 => (fv_te e1) \u (fv_te e2)
-  | trm_tabs V e1 => (fv_tt V) \u (fv_te e1)
+  | trm_tabs VS VU e1 => (fv_tt VS) \u (fv_tt VU) \u (fv_te e1)
   | trm_tapp e1 V => (fv_tt V) \u (fv_te e1)
   end.
 
@@ -300,7 +347,7 @@ Fixpoint fv_ee (e : trm) {struct e} : vars :=
   | trm_fvar x    => \{x}
   | trm_abs V e1  => (fv_ee e1)
   | trm_app e1 e2 => (fv_ee e1) \u (fv_ee e2)
-  | trm_tabs V e1 => (fv_ee e1)
+  | trm_tabs VS VU e1 => (fv_ee e1)
   | trm_tapp e1 V => (fv_ee e1)
   end.
 
@@ -309,10 +356,11 @@ Fixpoint fv_ee (e : trm) {struct e} : vars :=
 Fixpoint subst_tt (Z : var) (U : typ) (T : typ) {struct T} : typ :=
   match T with
   | typ_top         => typ_top
+  | typ_bot         => typ_bot
   | typ_bvar J      => typ_bvar J
   | typ_fvar X      => If X = Z then U else (typ_fvar X)
   | typ_arrow T1 T2 => typ_arrow (subst_tt Z U T1) (subst_tt Z U T2)
-  | typ_all T1 T2   => typ_all (subst_tt Z U T1) (subst_tt Z U T2)
+  | typ_all T0 T1 T2   => typ_all (subst_tt Z U T0) (subst_tt Z U T1) (subst_tt Z U T2)
   end.
 
 (** Substitution for free type variables in terms. *)
@@ -323,7 +371,7 @@ Fixpoint subst_te (Z : var) (U : typ) (e : trm) {struct e} : trm :=
   | trm_fvar x    => trm_fvar x
   | trm_abs V e1  => trm_abs  (subst_tt Z U V)  (subst_te Z U e1)
   | trm_app e1 e2 => trm_app  (subst_te Z U e1) (subst_te Z U e2)
-  | trm_tabs V e1 => trm_tabs (subst_tt Z U V)  (subst_te Z U e1)
+  | trm_tabs VS VU e1 => trm_tabs (subst_tt Z U VS) (subst_tt Z U VU)  (subst_te Z U e1)
   | trm_tapp e1 V => trm_tapp (subst_te Z U e1) (subst_tt Z U V)
   end.
 
@@ -335,7 +383,7 @@ Fixpoint subst_ee (z : var) (u : trm) (e : trm) {struct e} : trm :=
   | trm_fvar x    => If x = z then u else (trm_fvar x)
   | trm_abs V e1  => trm_abs V (subst_ee z u e1)
   | trm_app e1 e2 => trm_app (subst_ee z u e1) (subst_ee z u e2)
-  | trm_tabs V e1 => trm_tabs V (subst_ee z u e1)
+  | trm_tabs VS VU e1 => trm_tabs VS VU (subst_ee z u e1)
   | trm_tapp e1 V => trm_tapp (subst_ee z u e1) V
   end.
 
@@ -343,7 +391,7 @@ Fixpoint subst_ee (z : var) (u : trm) (e : trm) {struct e} : trm :=
 
 Definition subst_tb (Z : var) (P : typ) (b : bind) : bind :=
   match b with
-  | bind_sub T => bind_sub (subst_tt Z P T)
+  | bind_sub T0 T1 => bind_sub (subst_tt Z P T0) (subst_tt Z P T1)
   | bind_typ T => bind_typ (subst_tt Z P T)
   end.
 
@@ -355,7 +403,7 @@ Definition subst_tb (Z : var) (P : typ) (b : bind) : bind :=
 Hint Constructors type term wft ok okt value red.
 
 Hint Resolve
-  sub_top sub_refl_tvar sub_arrow
+  sub_top sub_bot sub_refl_tvar sub_arrow sub_refl_all
   typing_var typing_app typing_tapp typing_sub.
 
 (** Gathering free names already used in the proofs *)
@@ -389,7 +437,7 @@ Tactic Notation "apply_fresh" "*" constr(T) "as" ident(x) :=
 Ltac get_env :=
   match goal with
   | |- wft ?E _ => E
-  | |- sub ?E _ _  => E
+  | |- sub _ ?E _ _  => E
   | |- typing ?E _ _ => E
   end.
 
@@ -405,12 +453,19 @@ Tactic Notation "apply_empty" "*" constr(F) :=
 
 (** Tactic to undo when Coq does too much simplification *)
 
-Ltac unsimpl_map_bind :=
+Ltac unsimpl_map_bind_sub :=
+  match goal with |- context [ ?B (subst_tt ?Z ?P ?U0) (subst_tt ?Z ?P ?U1) ] =>
+    unsimpl ((subst_tb Z P) (B U0 U1)) end.
+
+Ltac unsimpl_map_bind_typ :=
   match goal with |- context [ ?B (subst_tt ?Z ?P ?U) ] =>
     unsimpl ((subst_tb Z P) (B U)) end.
 
-Tactic Notation "unsimpl_map_bind" "*" :=
-  unsimpl_map_bind; auto*.
+Tactic Notation "unsimpl_map_bind_sub" "*" :=
+  unsimpl_map_bind_sub; auto*.
+
+Tactic Notation "unsimpl_map_bind_typ" "*" :=
+  unsimpl_map_bind_typ; auto*.
 
 
 (* ********************************************************************** *)
@@ -696,66 +751,67 @@ Proof.
   intros. gen_eq K: (E & G). gen E F G.
   induction H; intros; subst; eauto.
   (* case: var *)
-  apply (@wft_var U). apply* binds_weaken.
+  apply (@wft_var T0 T1). apply* binds_weaken.
   (* case: all *)
-  apply_fresh* wft_all as Y. apply_ih_bind* H1.
+  apply_fresh* wft_all as Y. apply_ih_bind* H2.
 Qed.
 
 (** Through narrowing *)
 
-Lemma wft_narrow : forall V F U T E X,
-  wft (E & X ~<: V & F) T ->
-  ok (E & X ~<: U & F) ->
-  wft (E & X ~<: U & F) T.
+Lemma wft_narrow : forall V0 V1 F U0 U1 T E X,
+  wft (E & X ~ bind_sub V0 V1 & F) T ->
+  ok (E & X ~ bind_sub U0 U1 & F) ->
+  wft (E & X ~ bind_sub U0 U1 & F) T.
 Proof.
-  intros. gen_eq K: (E & X ~<: V & F). gen E F.
+  intros. gen_eq K: (E & X ~ bind_sub V0 V1 & F). gen E F.
   induction H; intros; subst; eauto.
   destruct (binds_middle_inv H) as [K|[K|K]]; try destructs K.
     applys wft_var. apply* binds_concat_right.
     subst. applys wft_var. apply~ binds_middle_eq.
     applys wft_var. apply~ binds_concat_left.
      apply* binds_concat_left.
-  apply_fresh* wft_all as Y. apply_ih_bind* H1.
+  apply_fresh* wft_all as Y. apply_ih_bind* H2.
 Qed.
 
 (** Through strengthening *)
 
 Lemma wft_strengthen : forall E F x U T,
- wft (E & x ~: U & F) T -> wft (E & F) T.
+ wft (E & x ~ bind_typ U & F) T -> wft (E & F) T.
 Proof.
-  intros. gen_eq G: (E & x ~: U & F). gen F.
+  intros. gen_eq G: (E & x ~ bind_typ U & F). gen F.
   induction H; intros F EQ; subst; auto.
-  apply* (@wft_var U0).
+  apply* (@wft_var T0 T1).
   destruct (binds_concat_inv H) as [?|[? ?]].
     apply~ binds_concat_right.
     destruct (binds_push_inv H1) as [[? ?]|[? ?]].
       subst. false.
       apply~ binds_concat_left.
   (* todo: binds_cases tactic *)
-  apply_fresh* wft_all as Y. apply_ih_bind* H1.
+  apply_fresh* wft_all as Y. apply_ih_bind* H2.
 Qed.
 
 (** Through type substitution *)
 
-Lemma wft_subst_tb : forall F Q E Z P T,
-  wft (E & Z ~<: Q & F) T ->
+Lemma wft_subst_tb : forall F Q0 Q1 E Z P T,
+  wft (E & Z ~ bind_sub Q0 Q1 & F) T ->
   wft E P ->
   ok (E & map (subst_tb Z P) F) ->
   wft (E & map (subst_tb Z P) F) (subst_tt Z P T).
 Proof.
-  introv WT WP. gen_eq G: (E & Z ~<: Q & F). gen F.
+  introv WT WP. gen_eq G: (E & Z ~ bind_sub Q0 Q1 & F). gen F.
   induction WT; intros F EQ Ok; subst; simpl subst_tt; auto.
   case_var*.
     apply_empty* wft_weaken.
     destruct (binds_concat_inv H) as [?|[? ?]].
-      apply (@wft_var (subst_tt Z P U)).
+      apply (@wft_var (subst_tt Z P T0) (subst_tt Z P T1)).
        apply~ binds_concat_right.
-       unsimpl_map_bind. apply~ binds_map.
+       unsimpl_map_bind_sub. apply binds_map.
+       assumption.
       destruct (binds_push_inv H1) as [[? ?]|[? ?]].
         subst. false~.
         applys wft_var. apply* binds_concat_left.
   apply_fresh* wft_all as Y.
-   unsimpl ((subst_tb Z P) (bind_sub T1)).
+   unsimpl ((subst_tb Z P) (bind_sub T0 T1)).
    lets: wft_type.
    rewrite* subst_tt_open_tt_var.
    apply_ih_map_bind* H0.
@@ -763,9 +819,9 @@ Qed.
 
 (** Through type reduction *)
 
-Lemma wft_open : forall E U T1 T2,
+Lemma wft_open : forall E U T0 T1 T2,
   ok E ->
-  wft E (typ_all T1 T2) ->
+  wft E (typ_all T0 T1 T2) ->
   wft E U ->
   wft E (open_tt T2 U).
 Proof.
@@ -792,8 +848,8 @@ Hint Extern 1 (ok _) => apply ok_from_okt.
 
 (** Extraction from a subtyping assumption in a well-formed environments *)
 
-Lemma wft_from_env_has_sub : forall x U E,
-  okt E -> binds x (bind_sub U) E -> wft E U.
+Lemma wft_from_env_has_sub : forall x U0 U1 E,
+  okt E -> binds x (bind_sub U0 U1) E -> wft E U0 /\ wft E U1.
 Proof.
   induction E using env_ind; intros Ok B.
   false* binds_empty_inv.
@@ -801,12 +857,12 @@ Proof.
     false (empty_push_inv H0).
     destruct (eq_push_inv H) as [? [? ?]]. subst. clear H.
      destruct (binds_push_inv B) as [[? ?]|[? ?]]. subst.
-       inversions H3. apply_empty* wft_weaken.
-       apply_empty* wft_weaken.
+       inversions H4. split; apply_empty* wft_weaken.
+       split; apply_empty* wft_weaken.
     destruct (eq_push_inv H) as [? [? ?]]. subst. clear H.
      destruct (binds_push_inv B) as [[? ?]|[? ?]]. subst.
        inversions H3.
-       apply_empty* wft_weaken.
+       split; apply_empty* wft_weaken.
 Qed.
 
 (** Extraction from a typing assumption in a well-formed environments *)
@@ -820,7 +876,7 @@ Proof.
     false (empty_push_inv H0).
     destruct (eq_push_inv H) as [? [? ?]]. subst. clear H.
      destruct (binds_push_inv B) as [[? ?]|[? ?]]. subst.
-       inversions H3.
+       inversions H4.
        apply_empty* wft_weaken.
     destruct (eq_push_inv H) as [? [? ?]]. subst. clear H.
      destruct (binds_push_inv B) as [[? ?]|[? ?]]. subst.
@@ -831,7 +887,7 @@ Qed.
 (** Extraction from a well-formed environment *)
 
 Lemma wft_from_okt_typ : forall x T E,
-  okt (E & x ~: T) -> wft E T.
+  okt (E & x ~ bind_typ T) -> wft E T.
 Proof.
   intros. inversions* H.
   false (empty_push_inv H1).
@@ -839,12 +895,12 @@ Proof.
   destruct (eq_push_inv H0) as [? [? ?]]. inversions~ H4.
 Qed.
 
-Lemma wft_from_okt_sub : forall x T E,
-  okt (E & x ~<: T) -> wft E T.
+Lemma wft_from_okt_sub : forall x T0 T1 E,
+  okt (E & x ~ bind_sub T0 T1) -> wft E T0 /\ wft E T1.
 Proof.
   intros. inversions* H.
   false (empty_push_inv H1).
-  destruct (eq_push_inv H0) as [? [? ?]]. inversions~ H4.
+  destruct (eq_push_inv H0) as [? [? ?]]. inversions~ H5.
   destruct (eq_push_inv H0) as [? [? ?]]. false.
 Qed.
 
@@ -870,7 +926,7 @@ Hint Resolve wft_subst_tb.
 (** Inversion lemma *)
 
 Lemma okt_push_inv : forall E X B,
-  okt (E & X ~ B) -> exists T, B = bind_sub T \/ B = bind_typ T.
+  okt (E & X ~ B) -> (exists T0 T1, B = bind_sub T0 T1) \/ (exists T, B = bind_typ T).
 Proof.
   introv O. inverts O.
     false* empty_push_inv.
@@ -878,8 +934,8 @@ Proof.
     lets (?&?&?): (eq_push_inv H). subst*.
 Qed.
 
-Lemma okt_push_sub_inv : forall E X T,
-  okt (E & X ~<: T) -> okt E /\ wft E T /\ X # E.
+Lemma okt_push_sub_inv : forall E X T0 T1,
+  okt (E & X ~ bind_sub T0 T1) -> okt E /\ wft E T0 /\ wft E T1 /\ X # E.
 Proof.
   introv O. inverts O.
     false* empty_push_inv.
@@ -887,12 +943,12 @@ Proof.
     lets (?&?&?): (eq_push_inv H). false.
 Qed.
 
-Lemma okt_push_sub_type : forall E X T,
-  okt (E & X ~<: T) -> type T.
-Proof. intros. applys wft_type. forwards*: okt_push_sub_inv. Qed.
+Lemma okt_push_sub_type : forall E X T0 T1,
+  okt (E & X ~ bind_sub T0 T1) -> type T0 /\ type T1.
+Proof. intros. split; applys wft_type; forwards*: okt_push_sub_inv. Qed.
 
 Lemma okt_push_typ_inv : forall E x T,
-  okt (E & x ~: T) -> okt E /\ wft E T /\ x # E.
+  okt (E & x ~ bind_typ T) -> okt E /\ wft E T /\ x # E.
 Proof.
   introv O. inverts O.
     false* empty_push_inv.
@@ -901,24 +957,24 @@ Proof.
 Qed.
 
 Lemma okt_push_typ_type : forall E X T,
-  okt (E & X ~: T) -> type T.
+  okt (E & X ~ bind_typ T) -> type T.
 Proof. intros. applys wft_type. forwards*: okt_push_typ_inv. Qed.
 
 Hint Immediate okt_push_sub_type okt_push_typ_type.
 
 (** Through narrowing *)
 
-Lemma okt_narrow : forall V (E F:env) U X,
-  okt (E & X ~<: V & F) ->
-  wft E U ->
-  okt (E & X ~<: U & F).
+Lemma okt_narrow : forall V0 V1 (E F:env) U0 U1 X,
+  okt (E & X ~ bind_sub V0 V1 & F) ->
+  wft E U0 -> wft E U1 ->
+  okt (E & X ~ bind_sub U0 U1 & F).
 Proof.
-  introv O W. induction F using env_ind.
+  introv O W0 W1. induction F using env_ind.
   rewrite concat_empty_r in *. lets*: (okt_push_sub_inv O).
   rewrite concat_assoc in *.
-   lets (T&[?|?]): okt_push_inv O; subst.
-     lets (?&?&?): (okt_push_sub_inv O).
-      applys~ okt_sub. applys* wft_narrow.
+   lets [[T0 [T1 Hsub]] | [T Htyp]]: (okt_push_inv O); subst.
+     lets (?&?&?&?): (okt_push_sub_inv O).
+      applys~ okt_sub; applys* wft_narrow.
      lets (?&?&?): (okt_push_typ_inv O).
       applys~ okt_typ. applys* wft_narrow.
 Qed.
@@ -926,23 +982,23 @@ Qed.
 (** Through strengthening *)
 
 Lemma okt_strengthen : forall x T (E F:env),
-  okt (E & x ~: T & F) ->
+  okt (E & x ~ bind_typ T & F) ->
   okt (E & F).
 Proof.
  introv O. induction F using env_ind.
   rewrite concat_empty_r in *. lets*: (okt_push_typ_inv O).
   rewrite concat_assoc in *.
-   lets (U&[?|?]): okt_push_inv O; subst.
-     lets (?&?&?): (okt_push_sub_inv O).
-      applys~ okt_sub. applys* wft_strengthen.
+   lets [[U0 [U1 Hsub]] | [U Htyp]]: (okt_push_inv O); subst.
+     lets (?&?&?&?): (okt_push_sub_inv O).
+      applys~ okt_sub; applys* wft_strengthen.
      lets (?&?&?): (okt_push_typ_inv O).
       applys~ okt_typ. applys* wft_strengthen.
 Qed.
 
 (** Through type substitution *)
 
-Lemma okt_subst_tb : forall Q Z P (E F:env),
-  okt (E & Z ~<: Q & F) ->
+Lemma okt_subst_tb : forall Q0 Q1 Z P (E F:env),
+  okt (E & Z ~ bind_sub Q0 Q1 & F) ->
   wft E P ->
   okt (E & map (subst_tb Z P) F).
 Proof.
@@ -950,9 +1006,9 @@ Proof.
   rewrite map_empty. rewrite concat_empty_r in *.
    lets*: (okt_push_sub_inv O).
   rewrite map_push. rewrite concat_assoc in *.
-   lets (U&[?|?]): okt_push_inv O; subst.
-     lets (?&?&?): (okt_push_sub_inv O).
-      applys~ okt_sub. applys* wft_subst_tb.
+   lets [[U0 [U1 Hsub]] | [U Htyp]]: (okt_push_inv O); subst.
+     lets (?&?&?&?): (okt_push_sub_inv O).
+      applys~ okt_sub; applys* wft_subst_tb.
      lets (?&?&?): (okt_push_typ_inv O).
       applys~ okt_typ. applys* wft_subst_tb.
 Qed.
@@ -973,13 +1029,14 @@ Proof.
  introv. unfold open_tt. generalize 0.
  induction T; simpl; intros k Fr; auto.
  specializes IHT1 k. specializes IHT2 k. auto.
- specializes IHT1 k. specializes IHT2 (S k). auto.
+ specializes IHT1 k. specializes IHT2 k. specializes IHT3 (S k). auto.
 Qed.
 
 Lemma notin_fv_wf : forall E X T,
   wft E T -> X # E -> X \notin fv_tt T.
 Proof.
   induction 1; intros Fr; simpl.
+  eauto.
   eauto.
   rewrite notin_singleton. intro. subst. applys binds_fresh_inv H Fr.
   notin_simpl; auto.
@@ -991,7 +1048,9 @@ Lemma map_subst_tb_id : forall G Z P,
 Proof.
   induction 1; intros Fr; autorewrite with rew_env_map; simpl.
   auto.
-  rewrite* <- IHokt. rewrite* subst_tt_fresh. apply* notin_fv_wf.
+  rewrite* <- IHokt.
+    rewrite* subst_tt_fresh. rewrite* subst_tt_fresh.
+    apply* notin_fv_wf. apply* notin_fv_wf.
   rewrite* <- IHokt. rewrite* subst_tt_fresh. apply* notin_fv_wf.
 Qed.
 
@@ -1001,13 +1060,18 @@ Qed.
 
 (** The subtyping relation is restricted to well-formed objects. *)
 
-Lemma sub_regular : forall E S T,
-  sub E S T -> okt E /\ wft E S /\ wft E T.
+Lemma sub_regular : forall m E S T,
+  sub m E S T -> okt E /\ wft E S /\ wft E T.
 Proof.
-  induction 1. auto*. auto*. auto*. jauto_set; auto. (* auto* too slow *)
-  split. auto*. split;
-   apply_fresh* wft_all as Y;
-    forwards~: (H1 Y); apply_empty* (@wft_narrow T1).
+  induction 1. auto*. auto*. auto*. auto*. auto*. jauto_set; auto. (* auto* too slow *)
+  auto*.
+  split. auto*.
+   inversion IHsub1 as [_ [HwfS0 HwfT0]].
+   inversion IHsub2 as [_ [HwfT1 HwfS1]].
+   split;
+   apply_fresh wft_all as Y; try assumption;
+   forwards~: (H3 Y); apply_empty* (@wft_narrow T0 T1).
+  auto*. auto*.
 Qed.
 
 (** The typing relation is restricted to well-formed objects. *)
@@ -1035,15 +1099,21 @@ Proof.
    apply_fresh* term_tabs as y.
      pick_fresh y. forwards~ K: (H0 y). destructs K.
        forwards*: okt_push_sub_inv.
+       inversion H5 as [_ [Hwf _]]. apply wft_type with (E:=E). assumption.
+     pick_fresh y. forwards~ K: (H0 y). destructs K.
+       forwards*: okt_push_sub_inv.
+       inversion H5 as [_ [_ [Hwf _]]]. apply wft_type with (E:=E). assumption.
      forwards~ K: (H0 y). destructs K. auto.
    apply_fresh* wft_all as Y.
+     pick_fresh y. forwards~ K: (H0 y). destructs K.
+      forwards*: okt_push_sub_inv.
      pick_fresh y. forwards~ K: (H0 y). destructs K.
       forwards*: okt_push_sub_inv.
      forwards~ K: (H0 Y). destructs K.
       forwards*: okt_push_sub_inv.
   splits*; destructs (sub_regular H0).
    apply* term_tapp. applys* wft_type.
-   applys* wft_open T1.
+   applys* wft_open T0 T1.
   splits*. destructs~ (sub_regular H0).
 Qed.
 
@@ -1069,23 +1139,23 @@ Qed.
 
 Hint Extern 1 (okt ?E) =>
   match goal with
-  | H: sub _ _ _ |- _ => apply (proj31 (sub_regular H))
+  | H: sub _ _ _ _ |- _ => apply (proj31 (sub_regular H))
   | H: typing _ _ _ |- _ => apply (proj31 (typing_regular H))
   end.
 
 Hint Extern 1 (wft ?E ?T) =>
   match goal with
   | H: typing E _ T |- _ => apply (proj33 (typing_regular H))
-  | H: sub E T _ |- _ => apply (proj32 (sub_regular H))
-  | H: sub E _ T |- _ => apply (proj33 (sub_regular H))
+  | H: sub _ E T _ |- _ => apply (proj32 (sub_regular H))
+  | H: sub _ E _ T |- _ => apply (proj33 (sub_regular H))
   end.
 
 Hint Extern 1 (type ?T) =>
   let go E := apply (@wft_type E); auto in
   match goal with
   | H: typing ?E _ T |- _ => go E
-  | H: sub ?E T _ |- _ => go E
-  | H: sub ?E _ T |- _ => go E
+  | H: sub _ ?E T _ |- _ => go E
+  | H: sub _ ?E _ T |- _ => go E
   end.
 
 Hint Extern 1 (term ?e) =>
@@ -1096,7 +1166,7 @@ Hint Extern 1 (term ?e) =>
   end.
 
 (***************************************************************************
-* Preservation and Progress for System-F with Subtyping - Proofs           *
+* Proofs                                                                   *
 ***************************************************************************)
 
 (** In parentheses are given the label of the corresponding
@@ -1109,29 +1179,36 @@ Hint Extern 1 (term ?e) =>
 (* ********************************************************************** *)
 (** Reflexivity (1) *)
 
-Lemma sub_reflexivity : forall E T,
+Lemma sub_reflexivity : forall m E T,
   okt E ->
   wft E T ->
-  sub E T T .
+  sub m E T T .
 Proof.
   introv Ok WI. lets W: (wft_type WI). gen E.
-  induction W; intros; inversions WI; eauto.
-  apply_fresh* sub_all as Y.
+  destruct m; induction W; intros; inversions WI; eauto using sub_trans_ok.
+  apply sub_arrow; apply sub_trans_ok; auto.
 Qed.
 
 (* ********************************************************************** *)
 (** Weakening (2) *)
 
-Lemma sub_weakening : forall E F G S T,
-   sub (E & G) S T ->
+Lemma sub_weakening : forall m E F G S T,
+   sub m (E & G) S T ->
    okt (E & F & G) ->
-   sub (E & F & G) S T.
+   sub m (E & F & G) S T.
 Proof.
   introv Typ. gen F. inductions Typ; introv Ok; auto.
   (* case: fvar trans *)
   apply* sub_trans_tvar. apply* binds_weaken.
+  (* case: fvar trans lower *)
+  apply sub_trans_tvar_lower with (T0:=T0) (T1:=T1); auto.
+  apply* binds_weaken.
   (* case: all *)
   apply_fresh* sub_all as Y. apply_ih_bind* H0.
+  (* case: trans_ok *)
+  apply* sub_trans_ok.
+  (* case: trans *)
+  apply* sub_trans.
 Qed.
 
 (* ********************************************************************** *)
@@ -1140,64 +1217,349 @@ Qed.
 Section NarrowTrans.
 
 Definition transitivity_on Q := forall E S T,
-  sub E S Q -> sub E Q T -> sub E S T.
+  sub oktrans E S Q -> sub oktrans E Q T -> sub oktrans E S T.
 
 Hint Unfold transitivity_on.
 
 Hint Resolve wft_narrow.
 
-Lemma sub_narrowing_aux : forall Q F E Z P S T,
-  transitivity_on Q ->
-  sub (E & Z ~<: Q & F) S T ->
-  sub E P Q ->
-  sub (E & Z ~<: P & F) S T.
+Lemma sub_narrowing_aux : forall Q0 Q1 m F E Z P0 P1 S T,
+  transitivity_on Q0 ->
+  transitivity_on Q1 ->
+  sub m (E & Z ~ bind_sub Q0 Q1 & F) S T ->
+  sub oktrans E Q0 P0 ->
+  sub oktrans E P1 Q1 ->
+  sub oktrans E P0 P1 ->
+  sub m (E & Z ~ bind_sub P0 P1 & F) S T.
 Proof.
-  introv TransQ SsubT PsubQ.
+  introv TransQ0 TransQ1 SsubT Q0subP0 P1subQ1 P0subP1.
   inductions SsubT; introv.
   apply* sub_top.
+  apply* sub_bot.
   apply* sub_refl_tvar.
   tests EQ: (X = Z).
-    lets M: (@okt_narrow Q).
-    apply (@sub_trans_tvar P).
-      asserts~ N: (ok (E & Z ~<: P & F)).
+    lets M: (@okt_narrow Q0 Q1).
+    apply (@sub_trans_tvar P0 P1).
+      asserts~ N: (ok (E & Z ~ bind_sub P0 P1 & F)).
        lets: ok_middle_inv_r N.
        apply~ binds_middle_eq.
-      apply TransQ.
+      do_rew* concat_assoc (apply_empty* sub_weakening).
+      apply TransQ1.
         do_rew* concat_assoc (apply_empty* sub_weakening).
-        binds_get H. auto*.
-    apply* (@sub_trans_tvar U). binds_cases H; auto.
+        binds_get H. inversion H0. subst. auto*.
+    apply* (@sub_trans_tvar T0 T1). binds_cases H; auto.
+  tests EQ: (X = Z).
+    lets M: (@okt_narrow Q0 Q1).
+    apply (@sub_trans_tvar_lower P0 P1).
+      asserts~ N: (ok (E & Z ~ bind_sub P0 P1 & F)).
+       lets: ok_middle_inv_r N.
+       apply~ binds_middle_eq.
+      do_rew* concat_assoc (apply_empty* sub_weakening).
+      apply TransQ0.
+        binds_get H. inversion H0. subst. auto*.
+        do_rew* concat_assoc (apply_empty* sub_weakening).
+    apply* (@sub_trans_tvar_lower T0 T1). binds_cases H; auto.
   apply* sub_arrow.
-  apply_fresh* sub_all as Y. apply_ih_bind* H0.
+  apply sub_refl_all.
+    apply* (@okt_narrow Q0 Q1).
+    apply* (@wft_narrow Q0 Q1).
+  apply_fresh* sub_all as Y. apply_ih_bind H0.
+    auto.
+    apply TransQ1.
+    apply TransQ0.
+    auto.
+    auto.
+    auto.
+    auto.
+  apply* sub_trans_ok.
+  apply *sub_trans.
 Qed.
 
 Lemma sub_transitivity : forall Q,
   transitivity_on Q.
 Proof.
-  intro Q. introv SsubQ QsubT. asserts* W: (type Q).
-  gen E S T. set_eq Q' EQ: Q. gen Q' EQ.
-  induction W; intros Q' EQ E S SsubQ;
-    induction SsubQ; try discriminate; inversions EQ;
-      intros T QsubT; inversions keep QsubT;
-        eauto 4 using sub_trans_tvar.
-  (* case: all / top -> only needed to fix well-formedness,
-     by building back what has been deconstructed too much *)
-  assert (sub E (typ_all S1 S2) (typ_all T1 T2)).
-    apply_fresh* sub_all as y.
-  auto*.
-  (* case: all / all *)
-  apply_fresh sub_all as Y. auto*.
-  applys~ (H0 Y). lets: (IHW T1).
-  apply_empty* (@sub_narrowing_aux T1).
+  intro Q. introv SsubQ QsubT.
+  apply* sub_trans.
 Qed.
 
-Lemma sub_narrowing : forall Q E F Z P S T,
-  sub E P Q ->
-  sub (E & Z ~<: Q & F) S T ->
-  sub (E & Z ~<: P & F) S T.
+Lemma sub_narrowing : forall Q0 Q1 m E F Z P0 P1 S T,
+  sub oktrans E Q0 P0 ->
+  sub oktrans E P1 Q1 ->
+  sub oktrans E P0 P1 ->
+  sub m (E & Z ~ bind_sub Q0 Q1 & F) S T ->
+  sub m (E & Z ~ bind_sub P0 P1 & F) S T.
 Proof.
   intros.
   apply* sub_narrowing_aux.
   apply* sub_transitivity.
+  apply* sub_transitivity.
+Qed.
+
+Inductive notvar : typ -> Prop :=
+  | notvar_top   : notvar typ_top
+  | notvar_bot   : notvar typ_bot
+  | notvar_arrow : forall T1 T2, notvar (typ_arrow T1 T2)
+  | notvar_all   : forall T0 T1 T2, notvar (typ_all T0 T1 T2).
+
+Hint Constructors notvar.
+
+Lemma sub_trans_notvar : forall E T1 T2 T3,
+  notvar T2 ->
+  sub notrans E T1 T2 ->
+  sub notrans E T2 T3 ->
+  sub notrans E T1 T3.
+Proof.
+  introv Hnotsel H12 H23.
+  inversion Hnotsel; subst.
+  - (* case top *)
+    inversion H23; subst.
+    + apply* sub_top.
+    + apply* sub_trans_tvar_lower.
+      apply* sub_trans. apply sub_trans_ok. assumption.
+  - (* case bot *)
+    inversion H12; subst.
+    + apply* sub_bot.
+    + apply* sub_trans_tvar.
+      apply* sub_trans. apply sub_trans_ok. assumption.
+  - (* case arrow *)
+    inversion H12; inversion H23; subst; auto.
+    + apply* sub_trans_tvar; eauto using sub_trans, sub_trans_ok.
+    + apply* sub_trans_tvar; eauto using sub_trans, sub_trans_ok.
+    + apply* sub_trans_tvar_lower; eauto using sub_trans, sub_trans_ok.
+    + apply* sub_arrow; eauto using sub_trans, sub_trans_ok.
+  - (* case all *)
+    inversion H12; inversion H23; subst; auto.
+    + apply* sub_trans_tvar; eauto using sub_trans, sub_trans_ok.
+    + apply* sub_trans_tvar; eauto using sub_trans, sub_trans_ok.
+    + apply* sub_trans_tvar_lower; eauto using sub_trans, sub_trans_ok.
+    + apply sub_all with (L:=L \u L0); eauto using sub_trans.
+      intros Y Fr.
+      apply sub_trans with (T2:=(T5 open_tt_var Y)).
+      assert ((E & Y ~ bind_sub T8 T9) = (E & Y ~ bind_sub T8 T9 & empty)) as A. {
+        rewrite concat_empty_r. reflexivity.
+      }
+      rewrite A.
+      apply* (@sub_narrowing T0 T4).
+      rewrite concat_empty_r.
+      eauto.
+      eauto.
+Qed.
+
+Inductive follow_ub : env -> typ -> typ -> Prop :=
+  | follow_ub_nil : forall E T,
+      wft E T ->
+      follow_ub E T T
+  | follow_ub_cons : forall E X Lo Hi T,
+      binds X (bind_sub Lo Hi) E ->
+      sub oktrans E Lo Hi ->
+      follow_ub E Hi T ->
+      follow_ub E (typ_fvar X) T.
+
+Inductive follow_lb : env -> typ -> typ -> Prop :=
+  | follow_lb_nil : forall E T,
+      wft E T ->
+      follow_lb E T T
+  | follow_lb_cons : forall E X Lo Hi T,
+      binds X (bind_sub Lo Hi) E ->
+      sub oktrans E Lo Hi ->
+      follow_lb E (typ_fvar X) T ->
+      follow_lb E Lo T.
+
+Hint Constructors follow_ub.
+Hint Constructors follow_lb.
+
+Lemma follow_lb_reg : forall E T1 T2,
+  follow_lb E T1 T2 ->
+  wft E T1 /\ wft E T2.
+Proof.
+  introv H. induction H.
+  auto.
+  split; auto.
+  inversion IHfollow_lb. assumption.
+Qed.
+
+Lemma invert_follow_lb : forall E T1 T2,
+  follow_lb E T1 T2 ->
+  T1 = T2 \/
+  exists X1 X2 Hi, (typ_fvar X2) = T2 /\
+    binds X1 (bind_sub T1 Hi) E /\
+    sub oktrans E T1 Hi /\
+    follow_lb E (typ_fvar X1) (typ_fvar X2).
+Proof.
+  intros.
+  induction H.
+  auto.
+  destruct IHfollow_lb as [IH | IH].
+  subst.
+  right. exists X X Hi. auto.
+  right.
+    destruct IH as [X1 [X2 [Hi' [Heq [IH1 [IH2 IH3]]]]]].
+    subst.
+    exists X X2 Hi. auto.
+Qed.
+
+Definition st_middle (E: env) (B C: typ) : Prop :=
+  B = C \/
+  sub notrans E typ_top C \/
+  (notvar B /\ sub notrans E B C).
+
+Definition chain (E: env) (A D: typ): Prop :=
+  (exists B C, follow_ub E A B /\ st_middle E B C /\ follow_lb E C D).
+
+Lemma empty_chain: forall E T, wft E T -> chain E T T.
+Proof.
+  intros.
+  unfold chain. unfold st_middle.
+  exists T T.
+  auto.
+Qed.
+
+Lemma chain3sub: forall E C1 C2 D,
+  sub notrans E C1 C2 ->
+  follow_lb E C2 D ->
+  sub notrans E C1 D.
+Proof.
+  introv Hst Hflb.
+  induction Hflb.
+  assumption.
+  apply IHHflb.
+  eapply sub_trans_tvar_lower; eauto using sub_trans_ok.
+Qed.
+
+Lemma chain2sub: forall E B1 B2 C D,
+  sub notrans E B1 B2 ->
+  st_middle E B2 C ->
+  follow_lb E C D ->
+  sub notrans E B1 D.
+Proof.
+  introv Hst Hm Hflb.
+  unfold st_middle in Hm.
+  destruct Hm as [Hm | [Hm | [Hm1 Hm2]]]; subst.
+  apply (chain3sub Hst Hflb).
+  apply chain3sub with (C2:=C).
+    apply sub_trans_notvar with (T2:=typ_top); auto.
+    apply Hflb.
+  apply chain3sub with (C2:=C).
+    apply sub_trans_notvar with (T2:=B2); auto.
+    apply Hflb.
+Qed.
+
+
+Lemma chain1sub: forall E A B C D,
+  okt E ->
+  follow_ub E A B ->
+  st_middle E B C ->
+  follow_lb E C D ->
+  sub notrans E A D.
+Proof.
+  introv Hok Hfub Hm Hflb.
+  induction Hfub.
+  apply chain2sub with (B2:=T) (C:=C); try assumption.
+    apply sub_reflexivity; auto.
+  apply* sub_trans_tvar.
+    apply sub_trans_ok.
+    apply* IHHfub.
+Qed.
+
+Lemma prepend_chain: forall E A1 A2 D,
+  sub oktrans E A1 A2 ->
+  chain E A2 D ->
+  chain E A1 D.
+Proof.
+  fix 5.
+  introv Hsub Hch.
+  unfold chain in *. unfold st_middle in *.
+  inversion Hsub; inversion H; subst.
+  - (* case top *)
+    destruct Hch as [B [C [Hch1 [Hch2 Hch3]]]].
+    inversion Hch1; subst.
+    destruct Hch2 as [Hch2 | [Hch2 | [Hch2a Hch2b]]]; subst.
+    + exists A1 typ_top. auto 10.
+    + exists A1 C. auto 10.
+    + exists A1 C. auto 10.
+  - (* case bot *)
+    destruct Hch as [B [C [Hch1 [Hch2 Hch3]]]].
+    exists typ_bot C.
+    assert (wft E C) as HwfC. {
+      apply follow_lb_reg in Hch3. inversion Hch3. assumption.
+    }
+    auto 10.
+  - (* case refl_tvar *)
+    assumption.
+  - (* case trans_tvar *)
+    set (IH := (prepend_chain E T3 A2 D H5 Hch)).
+    destruct IH as [B [C [IH1 [IH2 IH3]]]].
+    exists B C.
+    split.
+    eapply follow_ub_cons. eassumption. assumption. assumption.
+    split; assumption.
+  - (* case trans_tvar_lower *)
+    set (Hch' := Hch).
+    destruct Hch' as [B [C [Hch1 [Hch2 Hch3]]]].
+    inversion Hch1; subst.
+    + destruct Hch2 as [Hch2 | [Hch2 | [Hch2a Hch2b]]].
+      subst.
+      apply (prepend_chain E A1 T0 D H5).
+      exists T0 T0.
+      set (Hflb := (follow_lb_cons H0 H4 Hch3)).
+      auto.
+      exists A1 C.
+      splits.
+      apply follow_ub_nil. auto.
+      right. left. apply Hch2. apply Hch3.
+      inversion Hch2a.
+    + assert (bind_sub Lo Hi = bind_sub T0 T3) as Heq. {
+        eapply binds_func; eassumption.
+      }
+      inversions Heq.
+      apply (prepend_chain E A1 T0 D H5).
+      apply (prepend_chain E T0 T3 D H4).
+      exists B C.
+      splits.
+      assumption.
+      assumption.
+      assumption.
+  - (* case arrow *)
+    destruct Hch as [B [C [Hch1 [Hch2 Hch3]]]].
+    inversion Hch1; subst.
+    exists (typ_arrow S1 S2) C.
+    destruct Hch2 as [Hch2 | [Hch2 | [Hch2a Hch2b]]].
+    subst.
+    auto 10.
+    auto 10.
+    set (Hst := (sub_trans_notvar (notvar_arrow _ _) H Hch2b)).
+    auto 10.
+  - (* case refl_all *)
+    assumption.
+  - (* case all *)
+    destruct Hch as [B [C [Hch1 [Hch2 Hch3]]]].
+    inversion Hch1; subst.
+    exists (typ_all S0 S1 S2) C.
+    destruct Hch2 as [Hch2 | [Hch2 | [Hch2a Hch2b]]].
+    subst.
+    auto 10.
+    auto 10.
+    set (Hst := (sub_trans_notvar (notvar_all _ _ _) H Hch2b)).
+    auto 10.
+  - (* case trans_ok *)
+    apply (prepend_chain E _ _ _ H (prepend_chain E _ _ _ H0 Hch)).
+  - (* case trans *)
+    apply (prepend_chain E _ _ _ H (prepend_chain E _ _ _ H0 Hch)).
+Qed.
+
+Lemma sub_trans_pushback : forall E T1 T3,
+  sub oktrans E T1 T3 ->
+  sub notrans E T1 T3.
+Proof.
+  introv Hst.
+  inversion Hst; subst.
+  assumption.
+  assert (wft E T3) as HwfT3 by auto.
+  assert (okt E) as Hok by auto.
+  set (Hch := (prepend_chain H (prepend_chain H0 (empty_chain HwfT3)))).
+  unfold chain in Hch.
+  destruct Hch as [B [C [Hch1 [Hch2 Hch3]]]].
+  apply (chain1sub Hok Hch1 Hch2 Hch3).
 Qed.
 
 End NarrowTrans.
@@ -1205,34 +1567,52 @@ End NarrowTrans.
 (* ********************************************************************** *)
 (** Type substitution preserves subtyping (10) *)
 
-Lemma sub_through_subst_tt : forall Q E F Z S T P,
-  sub (E & Z ~<: Q & F) S T ->
-  sub E P Q ->
-  sub (E & map (subst_tb Z P) F) (subst_tt Z P S) (subst_tt Z P T).
+Lemma sub_through_subst_tt : forall Q0 Q1 m E F Z S T P,
+  sub m (E & Z ~ bind_sub Q0 Q1 & F) S T ->
+  sub oktrans E Q0 P ->
+  sub oktrans E P Q1 ->
+  sub m (E & map (subst_tb Z P) F) (subst_tt Z P S) (subst_tt Z P T).
 Proof.
-  introv SsubT PsubQ.
+  introv SsubT Q0subP PsubQ1.
   inductions SsubT; introv; simpl subst_tt.
   apply* sub_top.
+  apply* sub_bot.
   case_var.
     apply* sub_reflexivity.
     apply* sub_reflexivity.
      inversions H0. binds_cases H3.
-      apply* (@wft_var U).
-      apply* (@wft_var (subst_tt Z P U)). unsimpl_map_bind*.
-   case_var.
-    apply (@sub_transitivity Q).
+      apply* (@wft_var T0 T1).
+      apply* (@wft_var (subst_tt Z P T0) (subst_tt Z P T1)). unsimpl_map_bind_sub*.
+  case_var.
+    apply sub_trans_pushback. apply (@sub_transitivity Q1).
       apply_empty* sub_weakening.
-      rewrite* <- (@subst_tt_fresh Z P Q).
-        binds_get H. auto*.
+      rewrite* <- (@subst_tt_fresh Z P Q1).
+        binds_get H. inversion H0. subst. auto*.
         apply* (@notin_fv_wf E).
-    apply* (@sub_trans_tvar (subst_tt Z P U)).
+    apply* (@sub_trans_tvar (subst_tt Z P T0) (subst_tt Z P T1)).
       rewrite* (@map_subst_tb_id E Z P).
-        binds_cases H; unsimpl_map_bind*.
+        binds_cases H; unsimpl_map_bind_sub*.
+  case_var.
+    apply sub_trans_pushback. apply (@sub_transitivity Q0).
+      rewrite* <- (@subst_tt_fresh Z P Q0).
+        binds_get H. inversion H0. subst. auto*.
+        apply* (@notin_fv_wf E).
+      apply_empty* sub_weakening.
+    apply* (@sub_trans_tvar_lower (subst_tt Z P T0) (subst_tt Z P T1)).
+      rewrite* (@map_subst_tb_id E Z P).
+        binds_cases H; unsimpl_map_bind_sub*.
   apply* sub_arrow.
+  apply* sub_refl_all.
+   change (typ_all (subst_tt Z P T0) (subst_tt Z P T1) (subst_tt Z P T2))
+          with
+          (subst_tt Z P (typ_all T0 T1 T2)).
+   auto*.
   apply_fresh* sub_all as X.
-   unsimpl (subst_tb Z P (bind_sub T1)).
+   unsimpl (subst_tb Z P (bind_sub T0 T1)).
    do 2 rewrite* subst_tt_open_tt_var.
    apply_ih_map_bind* H0.
+  apply* sub_trans_ok.
+  apply* sub_trans.
 Qed.
 
 (* ********************************************************************** *)
@@ -1253,48 +1633,63 @@ Proof.
   apply* typing_app.
   apply_fresh* typing_tabs as X. forwards~ K: (H X).
    apply_ih_bind (H0 X); eauto.
-  apply* typing_tapp. apply* sub_weakening.
+   apply typing_regular in K.
+   inversion K as [HOK _].
+   apply wft_from_okt_sub in HOK.
+   inversion HOK as [HS HU].
+   apply okt_sub; auto.
+   apply* sub_weakening.
+  apply* typing_tapp; apply* sub_weakening.
   apply* typing_sub. apply* sub_weakening.
 Qed.
 
 (* ********************************************************************** *)
 (** Strengthening (6) *)
 
-Lemma sub_strengthening : forall x U E F S T,
-  sub (E & x ~: U & F) S T ->
-  sub (E & F) S T.
+Lemma sub_strengthening : forall x U m E F S T,
+  sub m (E & x ~ bind_typ U & F) S T ->
+  sub m (E & F) S T.
 Proof.
-  intros x U E F S T SsubT.
+  intros x U m E F S T SsubT.
   inductions SsubT; introv; auto* wft_strengthen.
   (* case: fvar trans *)
-  apply* (@sub_trans_tvar U0). binds_cases H; auto*.
+  apply* (@sub_trans_tvar T0 T1). binds_cases H; auto*.
+  (* case: fvar trans lower *)
+  apply* (@sub_trans_tvar_lower T0 T1). binds_cases H; auto*.
   (* case: all *)
   apply_fresh* sub_all as X. apply_ih_bind* H0.
+  (* case: trans_ok *)
+  apply* sub_trans_ok.
+  (* case: trans *)
+  apply* sub_trans.
 Qed.
 
 (************************************************************************ *)
 (** Preservation by Type Narrowing (7) *)
 
-Lemma typing_narrowing : forall Q E F X P e T,
-  sub E P Q ->
-  typing (E & X ~<: Q & F) e T ->
-  typing (E & X ~<: P & F) e T.
+Lemma typing_narrowing : forall Q0 Q1 E F X P0 P1 e T,
+  sub oktrans E Q0 P0 ->
+  sub oktrans E P1 Q1 ->
+  sub oktrans E P0 P1 ->
+  typing (E & X ~ bind_sub Q0 Q1 & F) e T ->
+  typing (E & X ~ bind_sub P0 P1 & F) e T.
 Proof.
-  introv PsubQ Typ. gen_eq E': (E & X ~<: Q & F). gen F.
+  introv Q0subP0 P1subQ1 P0subP1 Typ. gen_eq E': (E & X ~ bind_sub Q0 Q1 & F). gen F.
   inductions Typ; introv EQ; subst; simpl.
   binds_cases H0; apply* typing_var.
   apply_fresh* typing_abs as y. apply_ih_bind* H0.
   apply* typing_app.
   apply_fresh* typing_tabs as Y. apply_ih_bind* H0.
-  apply* typing_tapp. apply* (@sub_narrowing Q).
-  apply* typing_sub. apply* (@sub_narrowing Q).
+  apply* (@sub_narrowing Q0 Q1).
+  apply* typing_tapp; apply* (@sub_narrowing Q0 Q1).
+  apply* typing_sub. apply* (@sub_narrowing Q0 Q1).
 Qed.
 
 (************************************************************************ *)
 (** Preservation by Term Substitution (8) *)
 
 Lemma typing_through_subst_ee : forall U E F x T e u,
-  typing (E & x ~: U & F) e T ->
+  typing (E & x ~ bind_typ U & F) e T ->
   typing E u U ->
   typing (E & F) (subst_ee x u e) T.
 Proof.
@@ -1309,33 +1704,37 @@ Proof.
   apply_fresh* typing_tabs as Y.
     rewrite* subst_ee_open_te_var.
     apply_ih_bind* H0.
-  apply* typing_tapp. apply* sub_strengthening.
+  apply* sub_strengthening.
+  apply* typing_tapp; apply* sub_strengthening.
   apply* typing_sub. apply* sub_strengthening.
 Qed.
 
 (************************************************************************ *)
 (** Preservation by Type Substitution (11) *)
 
-Lemma typing_through_subst_te : forall Q E F Z e T P,
-  typing (E & Z ~<: Q & F) e T ->
-  sub E P Q ->
+Lemma typing_through_subst_te : forall Q0 Q1 E F Z e T P,
+  typing (E & Z ~ bind_sub Q0 Q1 & F) e T ->
+  sub oktrans E Q0 P ->
+  sub oktrans E P Q1 ->
   typing (E & map (subst_tb Z P) F) (subst_te Z P e) (subst_tt Z P T).
 Proof.
-  introv Typ PsubQ.
+  introv Typ Q0subP PsubQ1.
   inductions Typ; introv; simpls subst_tt; simpls subst_te.
   apply* typing_var. rewrite* (@map_subst_tb_id E Z P).
-   binds_cases H0; unsimpl_map_bind*.
+   binds_cases H0; unsimpl_map_bind_typ*.
   apply_fresh* typing_abs as y.
     unsimpl (subst_tb Z P (bind_typ V)).
     rewrite* subst_te_open_ee_var.
     apply_ih_map_bind* H0.
   apply* typing_app.
   apply_fresh* typing_tabs as Y.
-    unsimpl (subst_tb Z P (bind_sub V)).
+    unsimpl (subst_tb Z P (bind_sub VS VU)).
     rewrite* subst_te_open_te_var.
     rewrite* subst_tt_open_tt_var.
     apply_ih_map_bind* H0.
+    apply* sub_through_subst_tt.
   rewrite* subst_tt_open_tt. apply* typing_tapp.
+    apply* sub_through_subst_tt.
     apply* sub_through_subst_tt.
   apply* typing_sub. apply* sub_through_subst_tt.
 Qed.
@@ -1348,31 +1747,42 @@ Qed.
 
 Lemma typing_inv_abs : forall E S1 e1 T,
   typing E (trm_abs S1 e1) T ->
-  forall U1 U2, sub E T (typ_arrow U1 U2) ->
-     sub E U1 S1
+  forall U1 U2, sub notrans E T (typ_arrow U1 U2) ->
+     sub oktrans E U1 S1
   /\ exists S2, exists L, forall x, x \notin L ->
-     typing (E & x ~: S1) (e1 open_ee_var x) S2 /\ sub E S2 U2.
+     typing (E & x ~ bind_typ S1) (e1 open_ee_var x) S2 /\ sub oktrans E S2 U2.
 Proof.
   introv Typ. gen_eq e: (trm_abs S1 e1). gen S1 e1.
   induction Typ; intros S1 b1 EQ U1 U2 Sub; inversions EQ.
-  inversions* Sub. auto* (@sub_transitivity T).
+  inversions* Sub. auto* (@sub_transitivity T) sub_trans_ok sub_trans_pushback.
 Qed.
 
-Lemma typing_inv_tabs : forall E S1 e1 T,
-  typing E (trm_tabs S1 e1) T ->
-  forall U1 U2, sub E T (typ_all U1 U2) ->
-     sub E U1 S1
+Lemma typing_inv_tabs : forall E S10 S11 e1 T,
+  typing E (trm_tabs S10 S11 e1) T ->
+  forall U10 U11 U2, sub notrans E T (typ_all U10 U11 U2) -> sub oktrans E U10 U11 ->
+     sub oktrans E S10 U10 /\ sub oktrans E U11 S11
   /\ exists S2, exists L, forall X, X \notin L ->
-     typing (E & X ~<: U1) (e1 open_te_var X) (S2 open_tt_var X)
-     /\ sub (E & X ~<: U1) (S2 open_tt_var X) (U2 open_tt_var X).
+     typing (E & X ~ bind_sub U10 U11) (e1 open_te_var X) (S2 open_tt_var X)
+     /\ sub oktrans (E & X ~ bind_sub U10 U11) (S2 open_tt_var X) (U2 open_tt_var X).
 Proof.
-  intros E S1 e1 T H. gen_eq e: (trm_tabs S1 e1). gen S1 e1.
-  induction H; intros S1 b EQ U1 U2 Sub; inversion EQ.
-  inversions Sub. splits. auto.
+  intros E S10 S11 e1 T H. gen_eq e: (trm_tabs S10 S11 e1). gen S10 S11 e1.
+  induction H; intros S10 S11 b EQ U10 U11 U2 Sub SubU; inversion EQ.
+  inversions Sub.
+  subst. splits.
+   apply* sub_reflexivity.
+   apply* sub_reflexivity.
+   exists U2 L.
+   intros Y Fr. splits.
+   apply H; assumption.
+   specialize (H Y Fr).
+   apply typing_regular in H.
+   apply* sub_reflexivity.
+  splits.
+   auto. auto.
    exists T1. let L1 := gather_vars in exists L1.
    intros Y Fr. splits.
-    apply_empty* (@typing_narrowing S1). auto.
-  auto* (@sub_transitivity T).
+    apply_empty* (@typing_narrowing S10 S11). auto. auto.
+  auto* (@sub_transitivity T) sub_trans_ok sub_trans_pushback.
 Qed.
 
 (* ********************************************************************** *)
@@ -1393,15 +1803,15 @@ Proof.
        auto*.
   (* case: tapp *)
   inversions Red; try solve [ apply* typing_tapp ].
-  destruct~ (typing_inv_tabs Typ (U1:=T1) (U2:=T2)) as [P1 [S2 [L P2]]].
-    apply* sub_reflexivity.
+  destruct~ (typing_inv_tabs Typ (U10:=T0) (U11:=T1) (U2:=T2)) as [P1 [S20 [S21 [L P2]]]].
+    apply* (@sub_transitivity T).
     pick_fresh X. forwards~ K: (P2 X). destruct K.
      rewrite* (@subst_te_intro X).
      rewrite* (@subst_tt_intro X).
      (* todo: apply empty here *)
      asserts_rewrite (E = E & map (subst_tb X T) empty).
        rewrite map_empty. rewrite~ concat_empty_r.
-     apply* (@typing_through_subst_te T1).
+     apply* (@typing_through_subst_te T0 T1).
        rewrite* concat_empty_r.
   (* case sub *)
   apply* typing_sub.
@@ -1413,6 +1823,19 @@ Qed.
 (* ********************************************************************** *)
 (** Canonical Forms (14) *)
 
+Lemma value_not_bot : forall t T,
+  value t -> typing empty t T -> T <> typ_bot.
+Proof.
+  introv Val Typ. gen_eq E: (@empty bind).
+  induction Typ; introv EQE;
+    try solve [ inversion Val; congruence ].
+  apply sub_trans_pushback in H.
+  inversion H; subst; try solve [ congruence ].
+  induction T; try solve [ congruence ].
+  apply IHTyp; auto.
+  apply binds_empty_inv in H0. inversion H0.
+Qed.
+
 Lemma canonical_form_abs : forall t U1 U2,
   value t -> typing empty t (typ_arrow U1 U2) ->
   exists V, exists e1, t = trm_abs V e1.
@@ -1421,21 +1844,24 @@ Proof.
   gen_eq T: (typ_arrow U1 U2). gen U1 U2.
   induction Typ; introv EQT EQE;
    try solve [ inversion Val | inversion EQT | eauto ].
-    subst. inversion H.
+    subst. apply sub_trans_pushback in H. inversion H.
+      apply value_not_bot in Typ; try assumption. congruence.
       false (binds_empty_inv H0).
       inversions H0. forwards*: IHTyp.
 Qed.
 
-Lemma canonical_form_tabs : forall t U1 U2,
-  value t -> typing empty t (typ_all U1 U2) ->
-  exists V, exists e1, t = trm_tabs V e1.
+Lemma canonical_form_tabs : forall t U0 U1 U2,
+  value t -> typing empty t (typ_all U0 U1 U2) ->
+  exists V0 V1, exists e1, t = trm_tabs V0 V1 e1.
 Proof.
   introv Val Typ. gen_eq E: (@empty bind).
-  gen_eq T: (typ_all U1 U2). gen U1 U2.
+  gen_eq T: (typ_all U0 U1 U2). gen U0 U1 U2.
   induction Typ; introv EQT EQE;
    try solve [ inversion Val | inversion EQT | eauto ].
-    subst. inversion H.
+    subst. apply sub_trans_pushback in H. inversion H.
+      apply value_not_bot in Typ; try assumption. congruence.
       false* binds_empty_inv.
+      inversions H0. forwards*: IHTyp.
       inversions H0. forwards*: IHTyp.
 Qed.
 
@@ -1459,10 +1885,9 @@ Proof.
   left*.
   (* case: tapp *)
   right. destruct~ IHTyp as [Val1 | [e1' Rede1']].
-    destruct (canonical_form_tabs Val1 Typ) as [S [e3 EQ]].
+    destruct (canonical_form_tabs Val1 Typ) as [S0 [S1 [e3 EQ]]].
       subst. exists* (open_te e3 T).
       exists* (trm_tapp e1' T).
   (* case: sub *)
   auto*.
 Qed.
-
